cleanup; relocate helper lemmas and tactics from DownTo.v into more appropriate files

src/Examples/ECC/DownTo.v
@@ -1,4 +1,5 @@
 Require Import Rupicola.Lib.Api.
+Require Import Rupicola.Lib.SepLocals.
 
 Section Gallina.
   Definition downto'
@@ -8,133 +9,6 @@ Section Gallina.
              {state} init count (step:state->nat->state) : state :=
     downto' init 0 count step.
 End Gallina.
-
-
-(* TODO: move *)
-(* TODO: ideally, all compilation lemmas would now use seplogic for locals *)
-Section Var.
-  Context {semantics : Semantics.parameters}
-          {semantics_ok : Semantics.parameters_ok semantics}.
-
-  Definition Var (name : string) (value : word)
-    : Semantics.locals -> Prop :=
-    eq (map.put map.empty name value).
-
-  Lemma Var_get l name value R :
-    (Var name value * R)%sep l ->
-    map.get l name = Some value.
-  Proof.
-    destruct 1; cbv [Var] in *; cleanup.
-    match goal with H : map.split _ _ _ |- _ =>
-                    apply map.get_split with (k:=name) in H;
-                      destruct H; cleanup
-    end.
-    all:subst; autorewrite with mapsimpl in *.
-    all:congruence.
-  Qed.
-
-  Lemma Var_put_replace l n v v' (R : _ -> Prop) :
-    (Var n v * R)%sep l ->
-    (Var n v' * R)%sep (map.put l n v').
-  Proof.
-    destruct 1; cbv [Var] in *; cleanup.
-    match goal with H : map.split _ _ _ |- _ =>
-                    pose proof H;
-                    apply map.get_split with (k:=n) in H;
-                      destruct H; cleanup
-    end;
-      subst; autorewrite with mapsimpl in *; [ | congruence ].
-    do 2 eexists.
-    ssplit; [ | reflexivity | eassumption ].
-    cbv [map.split] in *; cleanup; subst.
-    ssplit; [ | eapply map.disjoint_put_l;
-                eauto using map.disjoint_empty_l ].
-    subst. rewrite map.putmany_comm by auto.
-    rewrite map.put_putmany_commute.
-    rewrite map.put_put_same.
-    apply map.putmany_comm.
-    eapply map.disjoint_put_r; eauto using map.disjoint_empty_r.
-  Qed.
-
-  Lemma Var_put_remove l n v (R : _ -> Prop) :
-    R (map.remove l n) ->
-    (Var n v * R)%sep (map.put l n v).
-  Proof.
-    intros.
-    do 2 eexists.
-    ssplit; [ | reflexivity | eassumption ].
-    cbv [map.split] in *; cleanup; subst.
-    ssplit; [ | eapply map.disjoint_put_l;
-                eauto using map.disjoint_empty_l, map.get_remove_same ].
-    rewrite map.putmany_comm
-      by (apply map.disjoint_put_l;
-          eauto using map.disjoint_empty_l, map.get_remove_same).
-    rewrite <-map.put_putmany_commute.
-    rewrite map.putmany_empty_r.
-    eapply map.map_ext; intros.
-    rewrite !map.get_put_dec, !map.get_remove_dec.
-    destruct_one_match; congruence.
-  Qed.
-
-  Lemma Var_put_undef l n v (R : Semantics.locals -> Prop) :
-    map.get l n = None ->
-    R l ->
-    (Var n v * R)%sep (map.put l n v).
-  Proof.
-    cbv [Var]; intros. do 2 eexists.
-    ssplit; [ | reflexivity | eassumption ].
-    eauto using map.split_undef_put.
-  Qed.
-
-  Lemma Var_exact n v :
-    Lift1Prop.iff1 (Var n v) (eq (map.put map.empty n v)).
-  Proof. reflexivity. Qed.
-
-  Lemma Var_put_eq_l l n v :
-    map.get l n = None ->
-    Lift1Prop.iff1 (eq l * Var n v)%sep (eq (map.put l n v)).
-  Proof.
-    repeat intro; cbv [Var sep].
-    split; intros; cleanup; subst.
-    { match goal with H : map.split _ _ (map.put map.empty _ _) |- _ =>
-                      apply map.split_put_r2l, map.split_empty_r in H;
-                        [ | autorewrite with mapsimpl; reflexivity ]
-      end.
-      congruence. }
-    { do 2 eexists. ssplit; [ | reflexivity .. ].
-      apply map.split_put_l2r, map.split_empty_r; eauto. }
-  Qed.
-
-  Lemma Var_put_eq_r l n v :
-    map.get l n = None ->
-    Lift1Prop.iff1 (Var n v * eq l)%sep (eq (map.put l n v)).
-  Proof.
-    rewrite sep_comm. apply Var_put_eq_l.
-  Qed.
-End Var.
-
-(* TODO: move *)
-Ltac extract_var H name :=
-  let l := match type of H with
-             sep _ _ ?l => l end in
-  let i := match type of H with
-             context [Var name ?i] => i end in
-  let R := fresh "R" in
-  let H' := fresh in
-  evar (R : Semantics.locals -> Prop);
-  assert ((Var name i * R)%sep l) as H' by ecancel_assumption;
-  subst R; clear H; rename H' into H.
-
-(* TODO : move *)
-Ltac straightline_locals :=
-  match goal with
-  | |- @map.get _ _ Semantics.locals _ _ = Some _ =>
-    eapply Var_get; ecancel_assumption
-  end.
-Ltac straightline' ::=
-  straightline_plus
-    ltac:(first [ straightline_locals
-                | straightline_map_solver ]).
 
 Section Compile.
   Context {semantics : Semantics.parameters}
@@ -154,7 +28,7 @@ Section Compile.
            | |- context [S (?x - 1)] =>
              replace (S (x-1)) with x by lia
            | H : (_ * _)%sep ?l |- _ (map.put ?l ?i_var _) =>
-             extract_var H i_var; eapply Var_put_replace in H;
+             extract_Var H i_var; eapply Var_put_replace in H;
              ecancel_assumption
            | _ => progress subst_lets_in_goal
            | _ => progress change 1%Z with (Z.of_nat 1)
@@ -169,59 +43,11 @@ Section Compile.
                   end
            end.
 
-  Local Ltac use_cmd_hyp :=
-    let H := lazymatch goal with
-             | H: context [WeakestPrecondition.cmd _ ?impl]
-               |- WeakestPrecondition.cmd _ ?impl _ _ _ _ => H end in
-    eapply Proper_cmd;
-    [ solve [apply Proper_call]
-    | repeat intro | eapply H ].
-
-  (* TODO: move *)
-  Lemma skipn_seq_step n start len :
-    skipn n (seq start len) = seq (start + n) (len - n).
-  Proof.
-    revert start len.
-    induction n; destruct len; cbn; try reflexivity.
-    { repeat (f_equal; try lia). }
-    { rewrite IHn.
-      repeat (f_equal; try lia). }
-  Qed.
-
-  (* TODO: move *)
-  Lemma fold_left_skipn_seq {A} i count (step :A -> _) init :
-    0 < i <= count ->
-    step (fold_left step (rev (skipn i (seq 0 count))) init) (i-1) =
-    fold_left step (rev (skipn (i-1) (seq 0 count))) init.
-  Proof.
-    intros. rewrite !skipn_seq_step, !Nat.add_0_l.
-    replace (count - (i - 1)) with (S (count - i)) by lia.
-    cbn [seq rev]. rewrite fold_left_app. cbn [fold_left].
-    replace (S (i-1)) with i by lia.
-    reflexivity.
-  Qed.
-
   Lemma downto'_step {A} i count (step :A -> _) init :
     0 < i <= count ->
     step (downto' init i count step) (i-1) = downto' init (i-1) count step.
   Proof.
     cbv [downto']; apply fold_left_skipn_seq.
-  Qed.
-
-  Definition fold_left_dependent
-             {A B C} (stepA : A -> C -> A) (stepB : A -> B -> C -> B)
-             cs initA initB :=
-    fold_left (fun ab c =>
-                 (stepA (fst ab) c, stepB (fst ab) (snd ab) c))
-              cs (initA, initB).
-  Lemma fold_left_dependent_fst {A B C} stepA stepB :
-    forall cs initA initB,
-      fst (@fold_left_dependent A B C stepA stepB cs initA initB) =
-      fold_left stepA cs initA.
-  Proof.
-    induction cs; intros; [ reflexivity | ].
-    cbn [fold_left fold_left_dependent fst snd].
-    erewrite <-IHcs. reflexivity.
   Qed.
 
   (* helper definition *)
@@ -245,8 +71,6 @@ Section Compile.
     = downto'_dependent initA initB (i-1) count stepA stepB.
   Proof. apply fold_left_skipn_seq. Qed.
 
-  (* TODO: find a better phrasing than step_locals *)
-  (* TODO: use separation logic for locals? *)
   Lemma compile_downto :
     forall (locals: Semantics.locals) (mem: Semantics.mem)
            (locals_ok : Semantics.locals -> Prop)
@@ -274,16 +98,6 @@ Section Compile.
          and-locals-post (Invl gst' (step st i) * Var i_var wi * Rl)%sep
          with-locals l and-memory m and-trace tr and-rest R'
          and-functions functions) ->
-      (*
-         WeakestPrecondition.cmd
-           (WeakestPrecondition.call functions)
-           step_impl tr m li
-           (fun tr' m' l' =>
-              tr = tr'
-              /\ (exists gst',
-                     (Invl (step st i) gst' * Var i_var wi * Rl)%sep l'
-                     /\ (Inv (step st i) gst' * R')%sep m'))) ->
-       *)
       (let head := v in
        (* continuation *)
        forall tr l m gst,
@@ -357,7 +171,7 @@ Section Compile.
         rewrite ?word.unsigned_of_Z_0, ?word.unsigned_of_Z_1;
         ssplit; try lia; [ | ].
       { repeat straightline'.
-        use_cmd_hyp;
+        use_hyp_with_matching_cmd;
           [ | try solve [handle_downto_locals] .. ].
         cbv [postcondition_norets postcondition_for] in *;
           cleanup; subst.
@@ -398,7 +212,7 @@ Section Compile.
         | H : context [downto'_dependent _ _ ?i] |- _ =>
           replace i with 0 in * by lia
         end.
-        use_cmd_hyp; subst_lets_in_goal; eauto. } }
+        use_hyp_with_matching_cmd; subst_lets_in_goal; eauto. } }
   Qed.
 
 End Compile.
