src/Lib/SepLocals.v
@@ -1,0 +1,125 @@
+Require Import Rupicola.Lib.Api.
+
+(* TODO: ideally, all compilation lemmas would now use seplogic for locals *)
+Section Var.
+  Context {semantics : Semantics.parameters}
+          {semantics_ok : Semantics.parameters_ok semantics}.
+
+  Definition Var (name : string) (value : word)
+    : Semantics.locals -> Prop :=
+    eq (map.put map.empty name value).
+
+  Lemma Var_get l name value R :
+    (Var name value * R)%sep l ->
+    map.get l name = Some value.
+  Proof.
+    destruct 1; cbv [Var] in *; cleanup.
+    match goal with H : map.split _ _ _ |- _ =>
+                    apply map.get_split with (k:=name) in H;
+                      destruct H; cleanup
+    end.
+    all:subst; autorewrite with mapsimpl in *.
+    all:congruence.
+  Qed.
+
+  Lemma Var_put_replace l n v v' (R : _ -> Prop) :
+    (Var n v * R)%sep l ->
+    (Var n v' * R)%sep (map.put l n v').
+  Proof.
+    destruct 1; cbv [Var] in *; cleanup.
+    match goal with H : map.split _ _ _ |- _ =>
+                    pose proof H;
+                    apply map.get_split with (k:=n) in H;
+                      destruct H; cleanup
+    end;
+      subst; autorewrite with mapsimpl in *; [ | congruence ].
+    do 2 eexists.
+    ssplit; [ | reflexivity | eassumption ].
+    cbv [map.split] in *; cleanup; subst.
+    ssplit; [ | eapply map.disjoint_put_l;
+                eauto using map.disjoint_empty_l ].
+    subst. rewrite map.putmany_comm by auto.
+    rewrite map.put_putmany_commute.
+    rewrite map.put_put_same.
+    apply map.putmany_comm.
+    eapply map.disjoint_put_r; eauto using map.disjoint_empty_r.
+  Qed.
+
+  Lemma Var_put_remove l n v (R : _ -> Prop) :
+    R (map.remove l n) ->
+    (Var n v * R)%sep (map.put l n v).
+  Proof.
+    intros.
+    do 2 eexists.
+    ssplit; [ | reflexivity | eassumption ].
+    cbv [map.split] in *; cleanup; subst.
+    ssplit; [ | eapply map.disjoint_put_l;
+                eauto using map.disjoint_empty_l, map.get_remove_same ].
+    rewrite map.putmany_comm
+      by (apply map.disjoint_put_l;
+          eauto using map.disjoint_empty_l, map.get_remove_same).
+    rewrite <-map.put_putmany_commute.
+    rewrite map.putmany_empty_r.
+    eapply map.map_ext; intros.
+    rewrite !map.get_put_dec, !map.get_remove_dec.
+    destruct_one_match; congruence.
+  Qed.
+
+  Lemma Var_put_undef l n v (R : Semantics.locals -> Prop) :
+    map.get l n = None ->
+    R l ->
+    (Var n v * R)%sep (map.put l n v).
+  Proof.
+    cbv [Var]; intros. do 2 eexists.
+    ssplit; [ | reflexivity | eassumption ].
+    eauto using map.split_undef_put.
+  Qed.
+
+  Lemma Var_exact n v :
+    Lift1Prop.iff1 (Var n v) (eq (map.put map.empty n v)).
+  Proof. reflexivity. Qed.
+
+  Lemma Var_put_eq_l l n v :
+    map.get l n = None ->
+    Lift1Prop.iff1 (eq l * Var n v)%sep (eq (map.put l n v)).
+  Proof.
+    repeat intro; cbv [Var sep].
+    split; intros; cleanup; subst.
+    { match goal with H : map.split _ _ (map.put map.empty _ _) |- _ =>
+                      apply map.split_put_r2l, map.split_empty_r in H;
+                        [ | autorewrite with mapsimpl; reflexivity ]
+      end.
+      congruence. }
+    { do 2 eexists. ssplit; [ | reflexivity .. ].
+      apply map.split_put_l2r, map.split_empty_r; eauto. }
+  Qed.
+
+  Lemma Var_put_eq_r l n v :
+    map.get l n = None ->
+    Lift1Prop.iff1 (Var n v * eq l)%sep (eq (map.put l n v)).
+  Proof.
+    rewrite sep_comm. apply Var_put_eq_l.
+  Qed.
+End Var.
+
+Ltac extract_Var H name :=
+  let l := match type of H with
+             sep _ _ ?l => l end in
+  let i := match type of H with
+             context [Var name ?i] => i end in
+  let R := fresh "R" in
+  let H' := fresh in
+  evar (R : Semantics.locals -> Prop);
+  assert ((Var name i * R)%sep l) as H' by ecancel_assumption;
+  subst R; clear H; rename H' into H.
+
+Ltac straightline_map_solver_locals :=
+  match goal with
+  | |- @map.get _ _ Semantics.locals _ _ = Some _ =>
+    eapply Var_get; ecancel_assumption
+  end.
+
+Ltac straightline' ::=
+  straightline_plus
+    ltac:(first [ straightline_map_solver_locals
+                | straightline_map_solver ]).
